

Taylor's Formula for $f(x,y)$ at $(0,0)$

Taylor's Formula for $f(x,y)$ at the Origin

$$\begin{aligned} f(x,y) = & f(0,0) + xf_x + yf_y + \frac{1}{2!}(x^2f_{xx} + 2xyf_{xy} + y^2f_{yy}) \\ & + \frac{1}{3!}(x^3f_{xxx} + 3x^2yf_{xxy} + 3xy^2f_{xyy} + y^3f_{yyy}) + \cdots + \frac{1}{n!} \left(x^n \frac{\partial^n f}{\partial x^n} + nx^{n-1}y \frac{\partial^n f}{\partial x^{n-1}\partial y} + \cdots + y^n \frac{\partial^n f}{\partial y^n} \right) \\ & + \frac{1}{(n+1)!} \left(x^{n+1} \frac{\partial^{n+1} f}{\partial x^{n+1}} + (n+1)x^ny \frac{\partial^{n+1} f}{\partial x^n \partial y} + \cdots + y^{n+1} \frac{\partial^{n+1} f}{\partial y^{n+1}} \right) \Big|_{(x,y)} \end{aligned}$$

EXAMPLE 1 Find a quadratic approximation to $f(x, y) = \sin x \sin y$ near the origin. How accurate is the approximation if $|x| \leq 0.1$ and $|y| \leq 0.1$?

Solution We take $n = 2$ in Equation (8):

$$\begin{aligned} f(x, y) = & f(0, 0) + (xf_x + yf_y) + \frac{1}{2}(x^2f_{xx} + 2xyf_{xy} + y^2f_{yy}) \\ & + \frac{1}{6}(x^3f_{xxx} + 3x^2yf_{xxy} + 3xy^2f_{xyy} + y^3f_{yyy}) \Big|_{(0,0)}. \end{aligned}$$

Calculating the values of the partial derivatives,

$$f(0, 0) = \sin x \sin y \Big|_{(0, 0)} = 0, \quad f_{xx}(0, 0) = -\sin x \sin y \Big|_{(0, 0)} = 0,$$

$$f_x(0, 0) = \cos x \sin y \Big|_{(0, 0)} = 0, \quad f_{xy}(0, 0) = \cos x \cos y \Big|_{(0, 0)} = 1,$$

$$f_y(0, 0) = \sin x \cos y \Big|_{(0, 0)} = 0, \quad f_{yy}(0, 0) = -\sin x \sin y \Big|_{(0, 0)} = 0,$$

we have the result

$$\sin x \sin y \approx 0 + 0 + 0 + \frac{1}{2} (x^2(0) + 2xy(1) + y^2(0)), \quad \text{or} \quad \sin x \sin y \approx xy.$$

Finding Quadratic and Cubic Approximations

In Exercises 1–10, use Taylor's formula for $f(x, y)$ at the origin to find quadratic and cubic approximations of f near the origin.

1. $f(x, y) = xe^y$

2. $f(x, y) = e^x \cos y$

3. $f(x, y) = y \sin x$

4. $f(x, y) = \sin x \cos y$

5. $f(x, y) = e^x \ln(1 + y)$

6. $f(x, y) = \ln(2x + y + 1)$

7. $f(x, y) = \sin(x^2 + y^2)$

8. $f(x, y) = \cos(x^2 + y^2)$

Answers

1. $f(x, y) = xe^y \Rightarrow f_x = e^y, f_y = xe^y, f_{xx} = 0, f_{xy} = e^y, f_{yy} = xe^y$
 $\Rightarrow f(x, y) \approx f(0, 0) + xf_x(0, 0) + yf_y(0, 0) + \frac{1}{2} [x^2 f_{xx}(0, 0) + 2xy f_{xy}(0, 0) + y^2 f_{yy}(0, 0)]$
 $= 0 + x \cdot 1 + y \cdot 0 + \frac{1}{2} (x^2 \cdot 0 + 2xy \cdot 1 + y^2 \cdot 0) = x + xy$ quadratic approximation;
 $f_{xxx} = 0, f_{xxy} = 0, f_{xyy} = e^y, f_{yyy} = xe^y$
 $\Rightarrow f(x, y) \approx \text{quadratic} + \frac{1}{6} [x^3 f_{xxx}(0, 0) + 3x^2 y f_{xxy}(0, 0) + 3xy^2 f_{xyy}(0, 0) + y^3 f_{yyy}(0, 0)]$
 $= x + xy + \frac{1}{6} (x^3 \cdot 0 + 3x^2 y \cdot 0 + 3xy^2 \cdot 1 + y^3 \cdot 0) = x + xy + \frac{1}{2} xy^2$, cubic approximation

Answers

2. $f(x, y) = e^x \cos y \Rightarrow f_x = e^x \cos y, f_y = -e^x \sin y, f_{xx} = e^x \cos y, f_{xy} = -e^x \sin y, f_{yy} = -e^x \cos y$
 $\Rightarrow f(x, y) \approx f(0, 0) + xf_x(0, 0) + yf_y(0, 0) + \frac{1}{2} [x^2 f_{xx}(0, 0) + 2xyf_{xy}(0, 0) + y^2 f_{yy}(0, 0)]$
 $= 1 + x \cdot 1 + y \cdot 0 + \frac{1}{2} [x^2 \cdot 1 + 2xy \cdot 0 + y^2 \cdot (-1)] = 1 + x + \frac{1}{2} (x^2 - y^2), \text{quadratic approximation;}$
 $f_{xxx} = e^x \cos y, f_{xxy} = -e^x \sin y, f_{xyy} = -e^x \cos y, f_{yyy} = e^x \sin y$
 $\Rightarrow f(x, y) \approx \text{quadratic} + \frac{1}{6} [x^3 f_{xxx}(0, 0) + 3x^2 y f_{xxy}(0, 0) + 3xy^2 f_{xyy}(0, 0) + y^3 f_{yyy}(0, 0)]$
 $= 1 + x + \frac{1}{2} (x^2 - y^2) + \frac{1}{6} [x^3 \cdot 1 + 3x^2 y \cdot 0 + 3xy^2 \cdot (-1) + y^3 \cdot 0]$
 $= 1 + x + \frac{1}{2} (x^2 - y^2) + \frac{1}{6} (x^3 - 3xy^2), \text{cubic approximation}$

Answers

3. $f(x, y) = y \sin x \Rightarrow f_x = y \cos x, f_y = \sin x, f_{xx} = -y \sin x, f_{xy} = \cos x, f_{yy} = 0$
 $\Rightarrow f(x, y) \approx f(0, 0) + xf_x(0, 0) + yf_y(0, 0) + \frac{1}{2} [x^2 f_{xx}(0, 0) + 2xy f_{xy}(0, 0) + y^2 f_{yy}(0, 0)]$
 $= 0 + x \cdot 0 + y \cdot 0 + \frac{1}{2} (x^2 \cdot 0 + 2xy \cdot 1 + y^2 \cdot 0) = xy$, quadratic approximation;
 $f_{xxx} = -y \cos x, f_{xxy} = -\sin x, f_{xyy} = 0, f_{yyy} = 0$
 $\Rightarrow f(x, y) \approx \text{quadratic} + \frac{1}{6} [x^3 f_{xxx}(0, 0) + 3x^2 y f_{xxy}(0, 0) + 3xy^2 f_{xyy}(0, 0) + y^3 f_{yyy}(0, 0)]$
 $= xy + \frac{1}{6} (x^3 \cdot 0 + 3x^2 y \cdot 0 + 3xy^2 \cdot 0 + y^3 \cdot 0) = xy$, cubic approximation

Answers

4. $f(x, y) = \sin x \cos y \Rightarrow f_x = \cos x \cos y, f_y = -\sin x \sin y, f_{xx} = -\sin x \cos y, f_{xy} = -\cos x \sin y,$
 $f_{yy} = -\sin x \cos y \Rightarrow f(x, y) \approx f(0, 0) + xf_x(0, 0) + yf_y(0, 0) + \frac{1}{2} [x^2 f_{xx}(0, 0) + 2xy f_{xy}(0, 0) + y^2 f_{yy}(0, 0)]$
 $= 0 + x \cdot 1 + y \cdot 0 + \frac{1}{2} (x^2 \cdot 0 + 2xy \cdot 0 + y^2 \cdot 0) = x$, quadratic approximation;
 $f_{xxx} = -\cos x \cos y, f_{xxy} = \sin x \sin y, f_{xyy} = -\cos x \cos y, f_{yyy} = \sin x \sin y$
 $\Rightarrow f(x, y) \approx \text{quadratic} + \frac{1}{6} [x^3 f_{xxx}(0, 0) + 3x^2 y f_{xxy}(0, 0) + 3xy^2 f_{xyy}(0, 0) + y^3 f_{yyy}(0, 0)]$
 $= x + \frac{1}{6} [x^3 \cdot (-1) + 3x^2 y \cdot 0 + 3xy^2 \cdot (-1) + y^3 \cdot 0] = x - \frac{1}{6} (x^3 + 3xy^2)$, cubic approximation

Answers

5. $f(x, y) = e^x \ln(1 + y) \Rightarrow f_x = e^x \ln(1 + y), f_y = \frac{e^x}{1+y}, f_{xx} = e^x \ln(1 + y), f_{xy} = \frac{e^x}{1+y}, f_{yy} = -\frac{e^x}{(1+y)^2}$
 $\Rightarrow f(x, y) \approx f(0, 0) + xf_x(0, 0) + yf_y(0, 0) + \frac{1}{2} [x^2 f_{xx}(0, 0) + 2xy f_{xy}(0, 0) + y^2 f_{yy}(0, 0)]$
 $= 0 + x \cdot 0 + y \cdot 1 + \frac{1}{2} [x^2 \cdot 0 + 2xy \cdot 1 + y^2 \cdot (-1)] = y + \frac{1}{2} (2xy - y^2)$, quadratic approximation;
 $f_{xxx} = e^x \ln(1 + y), f_{xxy} = \frac{e^x}{1+y}, f_{xyy} = -\frac{e^x}{(1+y)^2}, f_{yyy} = \frac{2e^x}{(1+y)^3}$
 $\Rightarrow f(x, y) \approx \text{quadratic} + \frac{1}{6} [x^3 f_{xxx}(0, 0) + 3x^2 y f_{xxy}(0, 0) + 3xy^2 f_{xyy}(0, 0) + y^3 f_{yyy}(0, 0)]$
 $= y + \frac{1}{2} (2xy - y^2) + \frac{1}{6} [x^3 \cdot 0 + 3x^2 y \cdot 1 + 3xy^2 \cdot (-1) + y^3 \cdot 2]$
 $= y + \frac{1}{2} (2xy - y^2) + \frac{1}{6} (3x^2 y - 3xy^2 + 2y^3)$, cubic approximation

Answers

6. $f(x, y) = \ln(2x + y + 1) \Rightarrow f_x = \frac{2}{2x + y + 1}, f_y = \frac{1}{2x + y + 1}, f_{xx} = \frac{-4}{(2x + y + 1)^2}, f_{xy} = \frac{-2}{(2x + y + 1)^2},$
 $f_{yy} = \frac{-1}{(2x + y + 1)^2} \Rightarrow f(x, y) \approx f(0, 0) + xf_x(0, 0) + yf_y(0, 0) + \frac{1}{2} [x^2 f_{xx}(0, 0) + 2xy f_{xy}(0, 0) + y^2 f_{yy}(0, 0)]$
 $= 0 + x \cdot 2 + y \cdot 1 + \frac{1}{2} [x^2 \cdot (-4) + 2xy \cdot (-2) + y^2 \cdot (-1)] = 2x + y + \frac{1}{2} (-4x^2 - 4xy - y^2)$
 $= (2x + y) - \frac{1}{2} (2x + y)^2$, quadratic approximation;
- $f_{xxx} = \frac{16}{(2x + y + 1)^3}, f_{xxy} = \frac{8}{(2x + y + 1)^3}, f_{xyy} = \frac{4}{(2x + y + 1)^3}, f_{yyy} = \frac{2}{(2x + y + 1)^3}$
 $\Rightarrow f(x, y) \approx \text{quadratic} + \frac{1}{6} [x^3 f_{xxx}(0, 0) + 3x^2 y f_{xxy}(0, 0) + 3xy^2 f_{xyy}(0, 0) + y^3 f_{yyy}(0, 0)]$
 $= (2x + y) - \frac{1}{2} (2x + y)^2 + \frac{1}{6} (x^3 \cdot 16 + 3x^2 y \cdot 8 + 3xy^2 \cdot 4 + y^3 \cdot 2)$
 $= (2x + y) - \frac{1}{2} (2x + y)^2 + \frac{1}{3} (8x^3 + 12x^2 y + 6xy^2 + y^3)$
 $= (2x + y) - \frac{1}{2} (2x + y)^2 + \frac{1}{3} (2x + y)^3$, cubic approximation

Answers

7. $f(x, y) = \sin(x^2 + y^2) \Rightarrow f_x = 2x \cos(x^2 + y^2), f_y = 2y \cos(x^2 + y^2), f_{xx} = 2 \cos(x^2 + y^2) - 4x^2 \sin(x^2 + y^2),$
 $f_{xy} = -4xy \sin(x^2 + y^2), f_{yy} = 2 \cos(x^2 + y^2) - 4y^2 \sin(x^2 + y^2)$
 $\Rightarrow f(x, y) \approx f(0, 0) + xf_x(0, 0) + yf_y(0, 0) + \frac{1}{2} [x^2 f_{xx}(0, 0) + 2xy f_{xy}(0, 0) + y^2 f_{yy}(0, 0)]$
 $= 0 + x \cdot 0 + y \cdot 0 + \frac{1}{2} (x^2 \cdot 2 + 2xy \cdot 0 + y^2 \cdot 2) = x^2 + y^2, \text{ quadratic approximation;}$
 $f_{xxx} = -12x \sin(x^2 + y^2) - 8x^3 \cos(x^2 + y^2), f_{xxy} = -4y \sin(x^2 + y^2) - 8x^2 y \cos(x^2 + y^2),$
 $f_{xyy} = -4x \sin(x^2 + y^2) - 8xy^2 \cos(x^2 + y^2), f_{yyy} = -12y \sin(x^2 + y^2) - 8y^3 \cos(x^2 + y^2)$
 $\Rightarrow f(x, y) \approx \text{quadratic} + \frac{1}{6} [x^3 f_{xxx}(0, 0) + 3x^2 y f_{xxy}(0, 0) + 3xy^2 f_{xyy}(0, 0) + y^3 f_{yyy}(0, 0)]$
 $= x^2 + y^2 + \frac{1}{6} (x^3 \cdot 0 + 3x^2 y \cdot 0 + 3xy^2 \cdot 0 + y^3 \cdot 0) = x^2 + y^2, \text{ cubic approximation}$

Answers

8. $f(x, y) = \cos(x^2 + y^2) \Rightarrow f_x = -2x \sin(x^2 + y^2), f_y = -2y \sin(x^2 + y^2),$
 $f_{xx} = -2 \sin(x^2 + y^2) - 4x^2 \cos(x^2 + y^2), f_{xy} = -4xy \cos(x^2 + y^2), f_{yy} = -2 \sin(x^2 + y^2) - 4y^2 \cos(x^2 + y^2)$
 $\Rightarrow f(x, y) \approx f(0, 0) + xf_x(0, 0) + yf_y(0, 0) + \frac{1}{2} [x^2 f_{xx}(0, 0) + 2xy f_{xy}(0, 0) + y^2 f_{yy}(0, 0)]$
 $= 1 + x \cdot 0 + y \cdot 0 + \frac{1}{2} [x^2 \cdot 0 + 2xy \cdot 0 + y^2 \cdot 0] = 1, \text{ quadratic approximation;}$
 $f_{xxx} = -12x \cos(x^2 + y^2) + 8x^3 \sin(x^2 + y^2), f_{xxy} = -4y \cos(x^2 + y^2) + 8x^2 y \sin(x^2 + y^2),$
 $f_{xyy} = -4x \cos(x^2 + y^2) + 8xy^2 \sin(x^2 + y^2), f_{yyy} = -12y \cos(x^2 + y^2) + 8y^3 \sin(x^2 + y^2)$
 $\Rightarrow f(x, y) \approx \text{quadratic} + \frac{1}{6} [x^3 f_{xxx}(0, 0) + 3x^2 y f_{xxy}(0, 0) + 3xy^2 f_{xyy}(0, 0) + y^3 f_{yyy}(0, 0)]$
 $= 1 + \frac{1}{6} (x^3 \cdot 0 + 3x^2 y \cdot 0 + 3xy^2 \cdot 0 + y^3 \cdot 0) = 1, \text{ cubic approximation}$